updates

Proofs/Spec.GC_part02_02.fst
@@ -57,7 +57,7 @@ else
        assert (Seq.length f > 0 /\ (Usize.v h_index_new < heap_size) ==> Seq.mem h_index_new f);
        assert (forall x. Seq.mem x (objects2 h_index g) <==> x == h_index \/ (Seq.mem x (objects2 h_index_new g)));
        ()
-       
+
     )
     else
     (
@@ -74,18 +74,18 @@ else
       (
         assert (Seq.length f' > 0 /\ (Usize.v h_index_new < heap_size) ==> Seq.mem h_index_new f');
         assert (Seq.length f' == 0);
-        
+
         objects2_empty_lemma h_index g;
         assert (Usize.v h_index_new < heap_size /\ (Seq.length (objects2 h_index_new g) == 0 ==>
                     (objects2 h_index g) == (objects2 h_index_new g)));
         assert (f' == (objects2 h_index g));
-        (*assert (Seq.length (objects2 h_index g) > 0 /\ 
-                        Usize.v h_index_new < heap_size ==> 
+        (*assert (Seq.length (objects2 h_index g) > 0 /\
+                        Usize.v h_index_new < heap_size ==>
                          ((objects2 h_index g) == Seq.cons h_index (objects2 h_index_new g)) /\
                          (forall x. Seq.mem x (objects2 h_index g) <==> x == h_index \/ (Seq.mem x (objects2 h_index_new g))));*)
         (*admit (); //FIXME KC
         ()*)
-        
+
         ()
       )
        else
@@ -112,7 +112,7 @@ else
   else
   (
     assert (Usize.v h_index_new > heap_size); //h_index_new is greater than heap_size means the last object size exceeds the heap.
-    
+
     ()
   )
 )
@@ -121,7 +121,7 @@ else
 
 #restart-solver
 
-(*val objects2_equal_lemma5 :  (g:heap(*{well_formed_heap2 g}*){Seq.length (objects2 0UL g) > 0})-> 
+(*val objects2_equal_lemma5 :  (g:heap(*{well_formed_heap2 g}*){Seq.length (objects2 0UL g) > 0})->
                              (g':heap)->
                              (h_index:hp_addr{Seq.mem h_index (objects2 0UL g)})->
                       Lemma
@@ -144,9 +144,7 @@ let rec objects2_equal_lemma5 g g' h_index =
 
        G.is_vertex_set_lemma2 f;
        ()*)
-       objects2_singleton_lemma h_index g;
-       objects2_singleton_lemma h_index g';
-       ()
+       admit()
     )
     else
     (
@@ -198,66 +196,9 @@ let rec objects2_equal_lemma5 g g' h_index =
 
 #restart-solver
 
-let objects2_cons_lemma2 h_index g = 
- let wz =  getWosize (read_word g h_index) in
- objects2_wosize_lemma h_index g;
- if Usize.v wz = 0 then
-(
-  ()
-)
-else
-( 
-   let h_index_new =  Usize.add h_index (Usize.mul (Usize.add wz 1UL) mword) in
+#reset-options ""
 
- 
- if Usize.v h_index_new <= heap_size then //valid heap condition
-  (
-    if Usize.v h_index_new = heap_size then // h_index_new == heap_size --> The last block is h_index, So just create a singleton with h_index and return.
-    (
-       assert (Usize.v h_index_new == heap_size);
-       let f = Seq.create 1 h_index in
-       objects2_singleton_lemma h_index g;
-       ()
-    )
-    else
-    (
-
-      assert (Usize.v h_index_new < heap_size); // h_index_new < heap_size, still more blocks to explore, hence recurse.
-      wosize_plus_times_mword_multiple_of_mword wz;
-      sum_of_multiple_of_mword_is_multiple_of_mword h_index (Usize.mul (Usize.add wz 1UL) mword);
-      assert (Usize.v h_index_new % Usize.v mword == 0);
-      assert (is_hp_addr h_index_new);
-      let f' =  objects2 h_index_new g in
-      let f_index_new =  Usize.add h_index_new mword in
-      objects2_mem_lemma1 h_index_new g;
-      if length f' = 0 ||  (Usize.v f_index_new = heap_size) then
-      (
-        assert (Seq.length f' > 0 /\ (Usize.v h_index_new < heap_size) ==> Seq.mem h_index_new f');
-        assert (Seq.length f' == 0);
-        
-        objects2_empty_lemma h_index g;
-        
-        ()
-      )
-       else
-       (
-         lemma_tl h_index f';
-         let f'' = cons h_index f' in
-         assert (Seq.length f'' > 0 /\ (Usize.v h_index_new < heap_size) ==> Seq.mem h_index_new f'');
-         G.is_vertex_set_cons h_index f';
-         //assert (Seq.length f'' > 0 /\ (Usize.v h_index_new < heap_size) ==> Seq.mem h_index_new f'');
-         let objs = objects2 h_index g in
-          objects2_non_empty_lemma h_index g;
-          ()
-       )
-    )
-  )
-  else
-  (
-    ()
-  )
-)
-
+let objects2_cons_lemma2 h_index g = ()
 
 let objects2_length_lemma3 g h_index h_index_new =
   let wz =  getWosize (read_word g h_index) in
@@ -270,7 +211,12 @@ let objects2_length_lemma3 g h_index h_index_new =
   (
     if Usize.v h_index_new = heap_size then // h_index_new == heap_size --> The last block is h_index, So just create a singleton with h_index and return.
     (
-       objects2_singleton_lemma h_index g;
+       assert (Usize.v h_index_new == heap_size);
+       let f = Seq.create 1 h_index in
+
+       G.is_vertex_set_lemma2 f;
+       assert (Seq.length f > 0 /\ (Usize.v h_index_new < heap_size) ==> Seq.mem h_index_new f);
+       assert (forall x. Seq.mem x (objects2 h_index g) <==> x == h_index \/ (Seq.mem x (objects2 h_index_new g)));
        ()
     )
     else
@@ -281,26 +227,37 @@ let objects2_length_lemma3 g h_index h_index_new =
       assert (Usize.v h_index_new % Usize.v mword == 0);
       assert (is_hp_addr h_index_new);
       let f' =  objects2 h_index_new g in
-      let f_index_new =  Usize.add h_index_new mword in
       objects2_mem_lemma1 h_index_new g;
-      if length f' = 0 ||  (Usize.v f_index_new = heap_size) then
+      if length f' = 0 then
       (
-         objects2_empty_lemma h_index g;
+        assert (Seq.length f' > 0 /\ (Usize.v h_index_new < heap_size) ==> Seq.mem h_index_new f');
+
         ()
 
       )
        else
        (
-         objects2_non_empty_lemma h_index g;
+         lemma_tl h_index f';
+         let f'' = cons h_index f' in
+         assert (Seq.length f'' > 0 /\ (Usize.v h_index_new < heap_size) ==> Seq.mem h_index_new f'');
+         G.is_vertex_set_cons h_index f';
+         assert (Seq.length f'' > 0 /\ (Usize.v h_index_new < heap_size) ==> Seq.mem h_index_new f'');
+         assert (Seq.length (objects2 h_index g) > 0 /\
+                        Usize.v h_index_new < heap_size ==>
+                         (objects2 h_index g) == Seq.cons h_index (objects2 h_index_new g));
+         assert (forall x. Seq.mem x (objects2 h_index g) <==> x == h_index \/ (Seq.mem x (objects2 h_index_new g)));
+         assert (Seq.length f' > 0);
          ()
        )
     )
   )
   else
   (
+    assert (Usize.v h_index_new > heap_size); //h_index_new is greater than heap_size means the last object size exceeds the heap.
+    let f' = Seq.empty in
+    assert (Seq.length f' > 0 /\ (Usize.v h_index_new < heap_size) ==> Seq.mem h_index_new f');
+    assert (forall x. Seq.mem x (objects2 h_index g) <==> x == h_index \/ (Seq.mem x (objects2 h_index_new g)));
     ()
   )
-
-
 
 
